(Im)mutable borrowing of refcells.
Other changes:
- Get rid of * spec pattern (deprecated in iris trunk)
- Make freeable_sz opaque (and simplifiy some proofs because of this)
- Refact option_as_mut and cell
- Prove lft_glb_acc, for gettings tokens of an intersections from tokens of its components
- Add some support for the = operator for ints in the proof mode

theories/typing/unsafe/refcell.v
@@ -1,3 +1,4 @@
+From Coq.QArith Require Import Qcanon.
 From iris.proofmode Require Import tactics.
 From iris.algebra Require Import auth csum frac agree.
 From iris.base_logic Require Import big_op fractional.
@@ -33,10 +34,10 @@ Section refcell_inv.
     (∃ st, l ↦ #(Z_of_refcell_st st) ∗ own γ (● st) ∗
       match st return _ with
       | None => &{α}(shift_loc l 1 ↦∗: ty.(ty_own) tid)
-      | Some (Cinr ({|agree_car := ν|}, q, n)) =>
-        ∃ q', ⌜(q + q')%Qp = 1%Qp⌝ ∗ q'.[ν] ∗
-              ty.(ty_shr) (α ∪ ν) tid (shift_loc l 1) ∗
-              ([†ν] ={lftE}=∗ &{α}(shift_loc l 1 ↦∗: ty.(ty_own) tid))
+      | Some (Cinr (agν, q, n)) =>
+        ∃ q' ν, agν ≡ to_agree ν ∗ ⌜(q + q')%Qp = 1%Qp⌝ ∗ q'.[ν] ∗
+                ty.(ty_shr) (α ∪ ν) tid (shift_loc l 1) ∗
+                (1.[ν] ={⊤, ⊤∖↑lftN}▷=∗ &{α}(shift_loc l 1 ↦∗: ty.(ty_own) tid))
       | Some _ => True
       end)%I.
 
@@ -44,7 +45,7 @@ Section refcell_inv.
     Proper (dist n ==> dist n) (refcell_inv tid l γ α).
   Proof.
     intros ty1 ty2 Hty. unfold refcell_inv.
-    repeat (f_contractive || f_equiv || apply Hty).
+    repeat (f_contractive || f_equiv || apply Hty || apply dist_S).
   Qed.
 
   Lemma refcell_inv_proper E L tid l γ α1 α2 ty1 ty2 :
@@ -63,12 +64,14 @@ Section refcell_inv.
       iSplit; iIntros "!>!#H"; iDestruct "H" as (vl) "[Hf H]"; iExists vl;
       iFrame; by iApply "Hown". }
     iDestruct "H" as (st) "H"; iExists st;
-      iDestruct "H" as "($&$&H)"; destruct st as [[|[[[]]]|]|]; try done;
+      iDestruct "H" as "($&$&H)"; destruct st as [[|[[]]|]|]; try done;
       last by iApply "Hb".
-    iDestruct "H" as (q') "(Heq & Htok & Hs & H†)". iExists q'. iFrame. iSplitL "Hs".
+    iDestruct "H" as (q' ν) "(Hag & Heq & Htok & Hs & Hh)". iExists q', ν.
+    iFrame. iSplitL "Hs".
     - iApply (ty_shr_mono); first done; last by iApply "Hshr".
       by iApply lft_glb_mono; [iApply Hα|iApply lft_incl_refl].
-    - iIntros "?". iApply ("Hb" with ">"). by iApply "H†".
+    - iIntros "H†". iMod ("Hh" with "H†") as "Hh". iModIntro. iNext. iMod "Hh".
+      by iApply "Hb".
   Qed.
 End refcell_inv.
 
@@ -104,29 +107,26 @@ Section refcell.
     iMod (bor_acc_cons with "LFT Hn Htok") as "[H Hclose]". done.
     iAssert ((q / 2).[κ] ∗ ▷ ∃ γ, refcell_inv tid l γ κ ty)%I with ">[-Hclose]"
       as "[$ HQ]"; last first.
-    { iMod ("Hclose" with "* HQ []") as "[Hb $]".
+    { iMod ("Hclose" with "HQ []") as "[Hb $]".
       - iIntros "!> H !>". iNext. iDestruct "H" as (γ st) "(? & _ & _)".
         iExists _. iIntros "{$H}!%". destruct st as [[|[[]?]|]|]; simpl; lia.
       - iMod (bor_exists with "LFT Hb") as (γ) "Hb". done.
         iExists κ, γ. iSplitR. by iApply lft_incl_refl. by iApply bor_na. }
     clear dependent n. iDestruct "H" as ([|n|[]]) "[Hn >%]"; try lia.
     - iFrame. iMod (own_alloc (● None)) as (γ) "Hst". done. iExists γ, None. by iFrame.
-    - iMod (lft_create with "LFT") as (ν) "[[Htok1 Htok2] _]". done.
+    - iMod (lft_create with "LFT") as (ν) "[[Htok1 Htok2] #Hhν]". done.
       iMod (own_alloc
          (● Some (Cinr (to_agree (ν : leibnizC _), (1/2)%Qp, n)))) as (γ) "Hst".
       { by apply auth_auth_valid. }
-      destruct (Qp_lower_bound (1/2) (q/2)) as (q' & q1 & q2 & H12 & ->). rewrite H12.
-      iDestruct "Htok'" as "[Htok' $]". iDestruct "Htok1" as "[Htok1 Htok1']".
-      iApply (fupd_mask_mono lftE). done.
       iMod (rebor _ _ (κ ∪ ν) with "LFT [] Hvl") as "[Hvl Hh]". done.
       { iApply lft_le_incl. apply gmultiset_union_subseteq_l. }
-      iMod (ty_share _ _ (κ ∪ ν) _ _ q' with "LFT Hvl [Htok' Htok1]")
-        as "[Hshr Htok]". done.
-      { rewrite -lft_tok_sep. iFrame. }
-      rewrite -lft_tok_sep. iDestruct "Htok" as "[$ Htok]".
-      iExists γ, _. iFrame "Hst Hn". iExists _. iIntros "{$Htok2 $Hshr}!>!>".
-      rewrite -H12 Qp_div_2. iSplit; first done. iIntros "H†". iApply "Hh".
-      rewrite -lft_dead_or. auto.
+      iDestruct (lft_glb_acc with "Htok' Htok1") as (q') "[Htok Hclose]".
+      iMod (ty_share with "LFT Hvl Htok") as "[Hshr Htok]". done.
+      iDestruct ("Hclose" with "Htok") as "[$ Htok]".
+      iExists γ, _. iFrame "Hst Hn". iExists _, _. iIntros "{$Htok2 $Hshr}!>!>".
+      rewrite Qp_div_2. iSplit; first done. iSplit; first done. iIntros "Hν".
+      iMod ("Hhν" with "Hν") as "Hν". iModIntro. iNext. iMod "Hν".
+      iApply fupd_mask_mono; last iApply "Hh". done. rewrite -lft_dead_or. auto.
     - iMod (own_alloc (● Some (Cinl (Excl ())))) as (γ) "Hst".
       { by apply auth_auth_valid. }
       iFrame. iExists _, _. by iFrame.
@@ -274,8 +274,6 @@ Section ref.
   Proof. intros. by eapply ref_proper. Qed.
 End ref.
 
-Definition refcell_refmutN := refcellN .@ "refmut".
-
 Section refmut.
   Context `{typeG Σ, refcellG Σ}.
   Local Hint Extern 1000 (_ ⊆ _) => set_solver : ndisj.
@@ -334,7 +332,7 @@ Section refmut.
     - iIntros "!# * % Htok".
       iMod (lft_incl_acc with "[] Htok") as (q') "[Htok Hclose]". set_solver.
       { iApply lft_glb_mono. iApply lft_incl_refl. done. }
-      iMod ("H" with "* [] Htok") as "Hshr". done. iModIntro. iNext.
+      iMod ("H" with "[] Htok") as "Hshr". done. iModIntro. iNext.
       iMod "Hshr" as "[Hshr Htok]". iMod ("Hclose" with "Htok") as "$".
       iApply ty_shr_mono; try done. iApply lft_glb_mono. iApply lft_incl_refl. done.
   Qed.
@@ -368,7 +366,7 @@ Section refmut.
       iDestruct "H" as "[$ #H]". iIntros "!# * % Htok".
       iMod (lft_incl_acc with "[] Htok") as (q') "[Htok Hclose]". set_solver.
       { iApply lft_glb_mono. done. iApply lft_incl_refl. }
-      iMod ("H" with "* [] Htok") as "Hshr". done. iModIntro. iNext.
+      iMod ("H" with "[] Htok") as "Hshr". done. iModIntro. iNext.
       iMod "Hshr" as "[Hshr Htok]". iMod ("Hclose" with "Htok") as "$".
       iApply ty_shr_mono; try done. iApply lft_glb_mono. done. iApply lft_incl_refl.
       by iApply "Hs".
@@ -405,32 +403,33 @@ Section refcell_functions.
 
   Lemma refcell_new_type ty :
     typed_instruction_ty [] [] [] (refcell_new ty)
-        (fn (λ _, [])%EL (λ _, [# ty]) (λ _:(), refcell ty)).
+        (fn (λ _, []) (λ _, [# ty]) (λ _:(), refcell ty)).
   Proof.
     apply type_fn; [apply _..|]. move=>/= _ ret arg. inv_vec arg=>x. simpl_subst.
     eapply type_new; [solve_typing..|].
     iIntros (r) "!# * #HEAP #LFT Hna HE HL Hk HT". simpl_subst.
     rewrite (Nat2Z.id (S ty.(ty_size))) tctx_interp_cons
             tctx_interp_singleton !tctx_hasty_val.
-    rewrite cctx_interp_singleton. iDestruct ("Hk" with "HE") as "Hret".
     iDestruct "HT" as "[Hr Hx]".
-    destruct x as [[]|]; try iDestruct "Hx" as "[]". iDestruct "Hx" as "[Hx Hx†]".
+    destruct x as [[|lx|]|]; try iDestruct "Hx" as "[]". iDestruct "Hx" as "[Hx Hx†]".
     iDestruct "Hx" as (vl) "[Hx↦ Hx]".
-    destruct r as [[]|]; try iDestruct "Hr" as "[]". iDestruct "Hr" as "[Hr Hr†]".
-    iDestruct "Hr" as (vl') "Hr". rewrite uninit_own. iDestruct "Hr" as "[Hr↦ >SZ]".
-    destruct vl' as [|]; iDestruct "SZ" as %[=]. rewrite heap_mapsto_vec_cons.
-    iDestruct "Hr↦" as "[Hr↦0 Hr↦1]". wp_op. rewrite shift_loc_0. wp_write. wp_op.
-    iDestruct (ty.(ty_size_eq) with "Hx") as %Hsz.
+    destruct r as [[|lr|]|]; try iDestruct "Hr" as "[]". iDestruct "Hr" as "[Hr Hr†]".
+    iDestruct "Hr" as (vl') "Hr". rewrite uninit_own.
+    iDestruct "Hr" as "[Hr↦ >SZ]". destruct vl' as [|]; iDestruct "SZ" as %[=].
+    rewrite heap_mapsto_vec_cons. iDestruct "Hr↦" as "[Hr↦0 Hr↦1]". wp_op.
+    rewrite shift_loc_0. wp_write. wp_op. iDestruct (ty.(ty_size_eq) with "Hx") as %Hsz.
     wp_bind (_ <-{_} !_)%E. iApply (wp_memcpy with "[$HEAP $Hr↦1 $Hx↦]"); [done..|].
-    iIntros "!> [Hr↦1 Hx↦]". wp_seq. wp_bind (delete _).
-    rewrite freeable_sz_full. iApply (wp_delete with "[$HEAP $Hx↦ Hx†]"); [by auto..| |].
-    { by rewrite Hsz. }
-    iIntros "!>_". wp_seq. iApply ("Hret" $! [# #_] with "Hna HL").
-    rewrite tctx_interp_singleton !tctx_hasty_val' //=. iFrame.
-    iExists (_::_). rewrite heap_mapsto_vec_cons. iFrame "Hr↦0 ∗". auto.
+    iIntros "!> [Hr↦1 Hx↦]". wp_seq.
+    iApply (type_delete _ _ [ #lx ◁ box (uninit (ty_size ty)); #lr ◁ box (refcell ty)]%TC
+        with "HEAP LFT Hna HE HL Hk [-]"); [solve_typing..| |]; last first.
+    { rewrite tctx_interp_cons tctx_interp_singleton !tctx_hasty_val' //=. iFrame.
+      iSplitL "Hx↦".
+      - iExists _. rewrite uninit_own. auto.
+      - iExists (_::_). rewrite heap_mapsto_vec_cons. iFrame. auto. }
+    eapply (type_jump [ #_]); solve_typing.
   Qed.
 
-  (* The other direction. *)
+  (* The other direction: getting ownership out of a refcell. *)
   Definition refcell_into_inner ty : val :=
     funrec: <> ["x"] :=
       let: "r" := new [ #ty.(ty_size)] in
@@ -439,29 +438,241 @@ Section refcell_functions.
 
   Lemma refcell_into_inner_type ty :
     typed_instruction_ty [] [] [] (refcell_into_inner ty)
-        (fn (λ _, [])%EL (λ _, [# refcell ty]) (λ _:(), ty)).
+        (fn (λ _, []) (λ _, [# refcell ty]) (λ _:(), ty)).
   Proof.
     apply type_fn; [apply _..|]. move=>/= _ ret arg. inv_vec arg=>x. simpl_subst.
     eapply type_new; [solve_typing..|].
     iIntros (r) "!# * #HEAP #LFT Hna HE HL Hk HT". simpl_subst.
     rewrite (Nat2Z.id (ty.(ty_size))) tctx_interp_cons
             tctx_interp_singleton !tctx_hasty_val.
-    rewrite cctx_interp_singleton. iDestruct ("Hk" with "HE") as "Hret".
-    iDestruct "HT" as "[Hr Hx]". destruct x as [[]|]; try iDestruct "Hx" as "[]".
-    iDestruct "Hx" as "[Hx Hx†]". rewrite freeable_sz_full.
+    iDestruct "HT" as "[Hr Hx]". destruct x as [[|lx|]|]; try iDestruct "Hx" as "[]".
+    iDestruct "Hx" as "[Hx Hx†]".
     iDestruct "Hx" as ([|[[]|]vl]) "[Hx↦ Hx]"; try iDestruct "Hx" as ">[]".
-    destruct r as [[]|]; try iDestruct "Hr" as "[]". iDestruct "Hr" as "[Hr Hr†]".
-    iDestruct "Hr" as (vl') "Hr". rewrite freeable_sz_full uninit_own heap_mapsto_vec_cons.
+    destruct r as [[|lr|]|]; try iDestruct "Hr" as "[]". iDestruct "Hr" as "[Hr Hr†]".
+    iDestruct "Hr" as (vl') "Hr". rewrite uninit_own heap_mapsto_vec_cons.
     iDestruct "Hr" as "[Hr↦ >%]". iDestruct "Hx↦" as "[Hx↦0 Hx↦1]". wp_op.
     iDestruct "Hx" as "[% Hx]". iDestruct (ty.(ty_size_eq) with "Hx") as %Hsz.
     wp_bind (_ <-{_} !_)%E. iApply (wp_memcpy with "[$HEAP $Hr↦ $Hx↦1]"); [done..|].
-    iIntros "!> [Hr↦ Hx↦1]". wp_seq. wp_bind (delete _).
-    iApply (wp_delete _ _ _ (_::_) with "[$HEAP Hx↦0 Hx↦1 Hx†]").
-    done. { by rewrite -Hsz. } { rewrite heap_mapsto_vec_cons -Hsz. iFrame. }
-    iIntros "!>_". wp_seq. iApply ("Hret" $! [# #_] with "Hna HL").
-    rewrite tctx_interp_singleton !tctx_hasty_val' //=. rewrite /= freeable_sz_full.
-    iFrame. iExists _. iFrame.
+    iIntros "!> [Hr↦ Hx↦1]". wp_seq.
+    iApply (type_delete _ _ [ #lx ◁ box (uninit (S (ty_size ty))); #lr ◁ box ty]%TC
+        with "HEAP LFT Hna HE HL Hk [-]"); [solve_typing..| |]; last first.
+    { rewrite tctx_interp_cons tctx_interp_singleton !tctx_hasty_val' //. iFrame.
+      iSplitR "Hr↦ Hx".
+      - iExists (_::_). rewrite heap_mapsto_vec_cons uninit_own -Hsz. iFrame. auto.
+      - iExists vl. iFrame. }
+    eapply (type_jump [ #_]); solve_typing.
   Qed.
 
+  Definition refcell_get_mut : val :=
+    funrec: <> ["x"] :=
+      let: "x'" := !"x" in
+      "x" <- "x'" +ₗ #1;;
+      "return" ["x"].
 
+  Lemma refcell_get_mut_type ty :
+    typed_instruction_ty [] [] [] refcell_get_mut
+        (fn (λ α, [☀α])%EL (λ α, [# &uniq{α} (refcell ty)])%T (λ α, &uniq{α} ty)%T).
+  Proof.
+    apply type_fn; [apply _..|]. move=>/= α ret arg. inv_vec arg=>x. simpl_subst.
+    eapply type_deref; [solve_typing..|by eapply read_own_move|done|]=>x'. simpl_subst.
+    iIntros "!# * #HEAP #LFT Hna HE HL HC HT".
+    rewrite tctx_interp_cons tctx_interp_singleton !tctx_hasty_val.
+    iDestruct "HT" as "[Hx Hx']". destruct x' as [[|lx'|]|];  try iDestruct "Hx'" as "[]".
+    iAssert (&{α} (∃ (z : Z), lx' ↦ #z ∗ ⌜-1 ≤ z⌝) ∗
+        (&uniq{α} ty).(ty_own) tid [ #(shift_loc lx' 1)])%I with ">[Hx']" as "[_ Hx']".
+    { iApply bor_sep; [done..|]. iApply (bor_proper with "Hx'"). iSplit.
+      - iIntros "[H1 H2]". iDestruct "H1" as (z) "[??]". iDestruct "H2" as (vl) "[??]".
+        iExists (_::_). rewrite heap_mapsto_vec_cons. iFrame. iFrame.
+      - iIntros "H". iDestruct "H" as ([|[[| |z]|]vl]) "[H↦ H]"; try iDestruct "H" as "[]".
+        rewrite heap_mapsto_vec_cons.
+        iDestruct "H" as "[H1 H2]". iDestruct "H↦" as "[H↦1 H↦2]".
+        iSplitL "H1 H↦1"; eauto. iExists _. iFrame. }
+    destruct x as [[|lx|]|]; try iDestruct "Hx" as "[]". iDestruct "Hx" as "[Hx Hx†]".
+    iDestruct "Hx" as (vl) "[Hx↦ Hx]". rewrite uninit_own. wp_op.
+    iApply (type_assign _ _ _ _
+            [ #lx ◁ box (uninit 1); #(shift_loc lx' 1) ◁ &uniq{α}ty]%TC
+            with "HEAP LFT Hna HE HL HC [-]");
+      [solve_typing..|by apply write_own| |]; last first.
+    { rewrite tctx_interp_cons tctx_interp_singleton !tctx_hasty_val' //. iFrame.
+      iNext. iExists _. rewrite uninit_own. iFrame. }
+    eapply (type_jump [ #_]); solve_typing.
+  Qed.
+
+  (* Shared borrowing. *)
+  Definition refcell_try_borrow : val :=
+    funrec: <> ["x"] :=
+      let: "r" := new [ #3 ] in
+      let: "x'" := !"x" in
+      let: "n" := !"x'" in
+      if: "n" ≤ #-1 then
+        "r" <-{Σ 1} ();;
+        "k" ["r"]
+      else
+        "x'" <- "n" + #1;;
+        let: "ref" := new [ #2 ] in
+        "ref" <- "x'" +ₗ #1;;
+        "ref" +ₗ #1 <- "x'";;
+        "r" <-{2,Σ 0} !"ref";;
+        delete [ #2; "ref"];;
+        "k" ["r"]
+      cont: "k" ["r"] :=
+        delete [ #1; "x"];; "return" ["r"].
+
+  Lemma refcell_try_borrow_type ty :
+    typed_instruction_ty [] [] [] refcell_try_borrow
+        (fn (λ α, [☀α])%EL (λ α, [# &shr{α}(refcell ty)]%T) (λ α, Σ[ref α ty; unit])%T).
+  Proof.
+    apply type_fn; [apply _..|]. move=>/= α ret arg. inv_vec arg=>x. simpl_subst.
+    eapply (type_cont [_] [] (λ r, [x ◁ box (&shr{α} refcell ty);
+                                    r!!!0 ◁ box Σ[ref α ty; unit]])%TC);
+      [solve_typing..|intros k|move=>/= k arg; inv_vec arg=>r]; simpl_subst; last first.
+    { eapply type_delete; [solve_typing..|].
+      eapply (type_jump [_]); solve_typing. }
+    eapply type_new; [solve_typing..|]=>r. simpl_subst.
+    eapply type_deref; [solve_typing..|apply read_own_copy, _|done|].
+    iIntros (x') "!# * #HEAP #LFT Hna HE HL Hk HT". simpl_subst.
+    rewrite 2!tctx_interp_cons tctx_interp_singleton !tctx_hasty_val.
+    iDestruct "HT" as "(Hx & Hx' & Hr)".
+    destruct x' as [[|lx|]|]; try iDestruct "Hx'" as "[]".
+    iDestruct "Hx'" as (β γ) "#[Hαβ Hinv]".
+    rewrite {1}/elctx_interp big_sepL_singleton.
+    iMod (lft_incl_acc with "Hαβ HE") as (qβ) "[[Hβtok1 Hβtok2] Hclose]". done.
+    iMod (na_bor_acc with "LFT Hinv Hβtok1 Hna") as "(INV & Hna & Hclose')"; try done.
+    iDestruct "INV" as (st) "(Hlx & Hownst & Hst)". wp_read. wp_let. wp_op=>?; wp_if.
+    - iMod ("Hclose'" with "[Hlx Hownst Hst] Hna") as "[Hβtok1 Hna]";
+        first by iExists st; iFrame.
+      iAssert (elctx_interp [☀α] qE)%I with ">[Hclose Hβtok1 Hβtok2]" as "HE".
+      { rewrite {1}/elctx_interp big_sepL_singleton /=. iApply "Hclose". by iFrame. }
+      iApply (type_sum_assign_unit [ref α ty; unit] _ _ _ _
+              [ x ◁ box (&shr{α}(refcell ty)); r ◁ box (uninit 3) ]%TC
+              with "HEAP LFT Hna HE HL Hk");
+        [solve_typing..|by eapply write_own|done| |]; first last.
+      { rewrite tctx_interp_cons tctx_interp_singleton !tctx_hasty_val. iFrame. }
+      simpl. eapply (type_jump [_]); solve_typing.
+    - wp_op. wp_write. wp_bind (new _). iApply wp_new; [done..|]. iNext.
+      iIntros (lref vl) "(EQ & H† & Hlref)". iDestruct "EQ" as %?%(inj Z.of_nat 2%nat).
+      destruct vl as [|?[|?[]]]; try done. wp_let.
+      rewrite heap_mapsto_vec_cons heap_mapsto_vec_singleton.
+      iDestruct "Hlref" as "[Hlref0 Hlref1]". wp_op. wp_write. wp_op. wp_write.
+      iAssert (∃ qν ν, (qβ / 2).[β] ∗ (qν).[ν] ∗
+                       ty_shr ty (β ∪ ν) tid (shift_loc lx 1) ∗
+                       own γ (◯ reading_st qν ν) ∗ refcell_inv tid lx γ β ty)%I
+        with ">[Hlx Hownst Hst Hβtok2]" as (q' ν) "(Hβtok2 & Hν & Hshr & Hreading & INV)".
+      { destruct st as [[|[[agν q] n]|]|]; try done.
+        - iDestruct "Hst" as (q' ν) "(Hag & #Hqq' & [Hν1 Hν2] & #Hshr & H†)".
+          iExists _, _. iFrame "Hν1". iDestruct "Hag" as %Hag. iDestruct "Hqq'" as %Hqq'.
+          iMod (own_update with "Hownst") as "[Hownst ?]".
+          { apply auth_update_alloc,
+               (op_local_update_discrete _ _ (reading_st (q'/2)%Qp ν))=>-[[Hagv _]_].
+            split; [split|].
+            - by rewrite -Hag /= agree_idemp.
+            - change ((q'/2+q)%Qp ≤ 1%Qp)%Qc. rewrite -Hqq' comm -{2}(Qp_div_2 q').
+              apply Qcplus_le_mono_l. rewrite -{1}(Qcplus_0_l (q'/2)%Qp).
+              apply Qcplus_le_mono_r, Qp_ge_0.
+            - done. }
+          iFrame "∗#". iExists _. rewrite Z.add_comm /=. iFrame. iExists _, _. iFrame.
+          rewrite /= Hag agree_idemp (comm Qp_plus) (assoc Qp_plus) Qp_div_2
+                  (comm Qp_plus). auto.
+        - iMod (lft_create with "LFT") as (ν) "[[Htok1 Htok2] #Hhν]". done.
+          iMod (own_update with "Hownst") as "[Hownst Hreading]"; first by apply
+            auth_update_alloc, (op_local_update_discrete _ _ (reading_st (1/2)%Qp ν)).
+          rewrite right_id. iExists _, _. iFrame "Htok1 Hreading".
+          iDestruct (lft_glb_acc with "Hβtok2 Htok2") as (q) "[Htok Hclose]".
+          iMod (rebor _ _ (β ∪ ν) with "LFT [] Hst") as "[Hst Hh]". done.
+          { iApply lft_le_incl. apply gmultiset_union_subseteq_l. }
+          iMod (ty_share with "LFT Hst Htok") as "[#Hshr Htok]". done. iFrame "Hshr".
+          iDestruct ("Hclose" with "Htok") as "[$ Htok2]". iExists _. iFrame.
+          iExists _, _. iFrame. rewrite Qp_div_2. iSplitR; first done. iSplitR; first done.
+          iIntros "{$Hshr} !> Hν". iMod ("Hhν" with "Hν") as "Hν". iModIntro.
+          iNext. iMod "Hν". iApply "Hh". rewrite -lft_dead_or. auto. }
+      iMod ("Hclose'" with "[$INV] Hna") as "[Hβtok1 Hna]".
+      iAssert (elctx_interp [☀α] qE)%I with ">[Hclose Hβtok1 Hβtok2]" as "HE".
+      { rewrite {1}/elctx_interp big_sepL_singleton /=. iApply "Hclose". by iFrame. }
+      iApply (type_sum_memcpy [ref α ty; unit] _ _ _ _ _ _ _ _
+        [ x ◁ box (&shr{α}(refcell ty)); r ◁ box (uninit 3); #lref ◁ box (ref α ty)]%TC
+              with "HEAP LFT Hna HE HL Hk");
+        [solve_typing..|by eapply write_own|by eapply read_own_move|done|done| |];
+        first last.
+      { rewrite 2!tctx_interp_cons tctx_interp_singleton !tctx_hasty_val. iFrame.
+        rewrite tctx_hasty_val' //. rewrite /= freeable_sz_full. iFrame.
+        iExists [_; _]. rewrite heap_mapsto_vec_cons heap_mapsto_vec_singleton.
+        iFrame. iExists _, _, _, _, _. iFrame "∗#". iApply ty_shr_mono; try by auto.
+        iApply lft_glb_mono. done. iApply lft_incl_refl. }
+      simpl. eapply type_delete; [solve_typing..|]. eapply (type_jump [_]); solve_typing.
+  Qed.
+
+  (* Unique borrowing. *)
+  Definition refcell_try_borrow_mut : val :=
+    funrec: <> ["x"] :=
+      let: "r" := new [ #3 ] in
+      let: "x'" := !"x" in
+      let: "n" := !"x'" in
+      if: "n" = #0 then
+        "x'" <- #(-1);;
+        let: "ref" := new [ #2 ] in
+        "ref" <- "x'" +ₗ #1;;
+        "ref" +ₗ #1 <- "x'";;
+        "r" <-{2,Σ 0} !"ref";;
+        delete [ #2; "ref"];;
+        "k" ["r"]
+      else
+        "r" <-{Σ 1} ();;
+        "k" ["r"]
+      cont: "k" ["r"] :=
+        delete [ #1; "x"];; "return" ["r"].
+
+  Lemma refcell_try_borrow_mut_type ty :
+    typed_instruction_ty [] [] [] refcell_try_borrow_mut
+        (fn (λ α, [☀α])%EL (λ α, [# &shr{α}(refcell ty)]%T) (λ α, Σ[refmut α ty; unit])%T).
+  Proof.
+    apply type_fn; [apply _..|]. move=>/= α ret arg. inv_vec arg=>x. simpl_subst.
+    eapply (type_cont [_] [] (λ r, [x ◁ box (&shr{α} refcell ty);
+                                    r!!!0 ◁ box Σ[refmut α ty; unit]])%TC);
+      [solve_typing..|intros k|move=>/= k arg; inv_vec arg=>r]; simpl_subst; last first.
+    { eapply type_delete; [solve_typing..|].
+      eapply (type_jump [_]); solve_typing. }
+    eapply type_new; [solve_typing..|]=>r. simpl_subst.
+    eapply type_deref; [solve_typing..|apply read_own_copy, _|done|].
+    iIntros (x') "!# * #HEAP #LFT Hna HE HL Hk HT". simpl_subst.
+    rewrite 2!tctx_interp_cons tctx_interp_singleton !tctx_hasty_val.
+    iDestruct "HT" as "(Hx & Hx' & Hr)".
+    destruct x' as [[|lx|]|]; try iDestruct "Hx'" as "[]".
+    iDestruct "Hx'" as (β γ) "#[Hαβ Hinv]".
+    rewrite {1}/elctx_interp big_sepL_singleton.
+    iMod (lft_incl_acc with "Hαβ HE") as (qβ) "[Hβtok Hclose]". done.
+    iMod (na_bor_acc with "LFT Hinv Hβtok Hna") as "(INV & Hna & Hclose')"; try done.
+    iDestruct "INV" as (st) "(Hlx & Hownst & Hst)". wp_read. wp_let. wp_op=>?; wp_if.
+    - wp_write. wp_bind (new _). iApply wp_new; [done..|]. iNext.
+      iIntros (lref vl) "(EQ & H† & Hlref)". iDestruct "EQ" as %?%(inj Z.of_nat 2%nat).
+      destruct vl as [|?[|?[]]]; try done. wp_let.
+      rewrite heap_mapsto_vec_cons heap_mapsto_vec_singleton.
+      iDestruct "Hlref" as "[Hlref0 Hlref1]". wp_op. wp_write. wp_op. wp_write.
+      destruct st as [[|[[]]|]|]; try done.
+      iMod (own_update with "Hownst") as "[Hownst ?]".
+      { apply auth_update_alloc, (op_local_update_discrete _ _ writing_st)=>//. }
+      iMod ("Hclose'" with "[Hlx Hownst] Hna") as "[Hβtok Hna]";
+        first by iExists _; iFrame.
+      iAssert (elctx_interp [☀α] qE)%I with ">[Hclose Hβtok]" as "HE".
+      { rewrite {1}/elctx_interp big_sepL_singleton /=. iApply "Hclose". by iFrame. }
+      iApply (type_sum_memcpy [refmut α ty; unit] _ _ _ _ _ _ _ _
+        [ x ◁ box (&shr{α}(refcell ty)); r ◁ box (uninit 3); #lref ◁ box (refmut α ty)]%TC
+              with "HEAP LFT Hna HE HL Hk");
+        [solve_typing..|by eapply write_own|by eapply read_own_move|done|done| |];
+        first last.
+      { rewrite 2!tctx_interp_cons tctx_interp_singleton !tctx_hasty_val. iFrame.
+        rewrite tctx_hasty_val' //. rewrite /= freeable_sz_full. iFrame.
+        iExists [_; _]. rewrite heap_mapsto_vec_cons heap_mapsto_vec_singleton.
+        iFrame. iExists _, _, _. iFrame "∗#". }
+      simpl. eapply type_delete; [solve_typing..|]. eapply (type_jump [_]); solve_typing.
+    - iMod ("Hclose'" with "[Hlx Hownst Hst] Hna") as "[Hβtok Hna]";
+        first by iExists st; iFrame.
+      iAssert (elctx_interp [☀α] qE)%I with ">[Hclose Hβtok]" as "HE".
+      { rewrite {1}/elctx_interp big_sepL_singleton /=. iApply "Hclose". by iFrame. }
+      iApply (type_sum_assign_unit [refmut α ty; unit] _ _ _ _
+              [ x ◁ box (&shr{α}(refcell ty)); r ◁ box (uninit 3) ]%TC
+              with "HEAP LFT Hna HE HL Hk");
+        [solve_typing..|by eapply write_own|done| |]; first last.
+      { rewrite tctx_interp_cons tctx_interp_singleton !tctx_hasty_val. iFrame. }
+      simpl. eapply (type_jump [_]); solve_typing.
+  Qed.
 End refcell_functions.
