theories/lifetime/frac_borrow.v
@@ -42,13 +42,13 @@ Section frac_bor.
     iIntros (?) "#LFT Hφ". iMod (own_alloc 1%Qp) as (γ) "?". done.
     iMod (bor_acc_atomic_strong with "LFT Hφ") as "[H|[H† Hclose]]". done.
     - iDestruct "H" as (κ') "(#Hκκ' & Hφ & Hclose)".
-      iMod ("Hclose" with "*[-] []") as "Hφ"; last first.
+      iMod ("Hclose" with "[-] []") as "Hφ"; last first.
       { iExists γ, κ'. iFrame "#". iApply (bor_share with "Hφ"). done. }
       { iIntros "!>Hφ H†!>". iNext. iDestruct "Hφ" as (q') "(Hφ & _ & [%|Hκ])". by subst.
         iDestruct "Hκ" as (q'') "[_ Hκ]".
         iDestruct (lft_tok_dead with "Hκ H†") as "[]". }
       iExists 1%Qp. iFrame. eauto.
-    - iMod ("Hclose" with "*") as "_"; last first.
+    - iMod "Hclose" as "_"; last first.
       iExists γ, κ. iSplitR. by iApply lft_incl_refl.
       iMod (bor_fake with "LFT H†"). done. by iApply bor_share.
   Qed.
